simplified sim relation that does not track the entire physical state, just the call id stacks

theories/sim/local.v
@@ -115,6 +115,11 @@ Qed.
   - We start after the substitution.
   - We assume the arguments are values related by [r]
   - The returned result must also be values and related by [vrel]. *)
+Definition fun_post (esat: A → state → state → Prop) initial_call_id_stack
+  (r: A) (n: nat) rs σs rt σt :=
+  (∃ c, σt.(scs) = c :: initial_call_id_stack) ∧
+  esat r σs σt ∧
+  (∃ vs vt, rs = ValR vs ∧ rt = ValR vt ∧ vrel r vs vt).
 Definition sim_local_fun
   (esat: A → state → state → Prop) (fn_src fn_tgt : function) : Prop :=
   ∀ r es et (vl_src vl_tgt: list value) σs σt
@@ -123,16 +128,12 @@ Definition sim_local_fun
     (EQT: subst_l fn_tgt.(fun_b) (Val <$> vl_tgt) fn_tgt.(fun_e) = Some et),
     ∃ idx, sim_local_body r idx
                           (InitCall es) σs (InitCall et) σt
-                          (λ r' _ rs' σs' rt' σt',
-                            (∃ c, σt'.(scs) = c :: σt.(scs)) ∧
-                            esat r' σs' σt' ∧
-                            (∃ vs' vt', rs' = ValR vs' ∧ rt' = ValR vt' ∧
-                               vrel r' vs' vt')).
+                          (fun_post esat σt.(scs)).
 
 Definition sim_local_funs (esat: A → state → state → Prop) : Prop :=
   ∀ name fn_tgt, fnt !! name = Some fn_tgt → ∃ fn_src,
     fns !! name = Some fn_src ∧
-    length (fn_src.(fun_b)) = length (fn_tgt.(fun_b)) ∧
+    length fn_src.(fun_b) = length fn_tgt.(fun_b) ∧
     sim_local_fun esat fn_src fn_tgt.
 
 End local.
